sub environments

deps/poulet4/lib/P4cub/Envn.v
@@ -61,6 +61,13 @@ Section EnvDefs.
       end
     end.
 
+  Definition sub_env (e1 e2 : t D T) : Prop :=
+    forall k v,
+      find k e1 = Some v -> find k e2 = Some v.
+
+  Definition eq_env (e1 e2 : t D T) : Prop :=
+    sub_env e1 e2 /\ sub_env e2 e1.
+  
   Section Lemmas.
     Local Hint Extern 0 => simpl_equiv_dec : core.
     Local Hint Extern 0 => simpl_equiv_dec_hyp : core.
@@ -93,6 +100,116 @@ Section EnvDefs.
       assert (equiv_rel x z) by (symmetry; assumption).
       assert (equiv_rel x y) by (etransitivity; eauto).
       contradiction.
+    Qed.
+
+    Lemma in_keys_find : forall e k,
+        In k (keys e) -> exists v, find k e = Some v.
+    Proof.
+      induction e as [| [k vl] e IHe];
+        intros ky Hky; simpl in *; try contradiction.
+      destruct (HE ky k); unravel in *; eauto.
+      destruct (find k e) as [v' |] eqn:Hfind;
+        unravel in *; intuition; subst; intuition.
+    Qed.
+
+    Lemma find_in_keys : forall e k v,
+        find k e = Some v -> exists k', equiv_rel k k' /\ In k' (keys e).
+    Proof.
+      intro e; induction e as [| [k v] e IHe];
+        intros ky vl Hkyvl; simpl in *; try discriminate.
+      destruct (HE ky k); unravel in *.
+      - inv Hkyvl.
+        destruct (find k e) as [v' |] eqn:Hfind.
+        + apply IHe in Hfind as (k' & Hkk' & HInk').
+          exists k'. intuition. transitivity k; assumption.
+        + exists k. intuition.
+      - destruct (find k e) as [v' |] eqn:Hfind;
+          apply IHe in Hkyvl as (k' & Hkk' & HInk'); firstorder.
+    Qed.
+
+    Lemma find_equiv_rel : forall e k1 k2,
+        equiv_rel k1 k2 -> find k1 e = find k2 e.
+    Proof.
+      intro e; induction e as [| [k v] e IHe];
+        intros k1 k2 Heq; simpl in *; auto.
+      destruct (HE k1 k) as [Hk1k | Hk1k];
+        destruct (HE k2 k) as [Hk2k | Hk2k];
+        unravel in *;
+        try (rewrite Heq in Hk1k; contradiction);
+        auto.
+    Qed.
+
+    Lemma find_none_not_in_keys : forall e k,
+        find k e = None -> ~ In k (keys e).
+    Proof.
+      intros e k Hfind Hin.
+      apply in_keys_find in Hin as (v & Hv).
+      rewrite Hfind in Hv. discriminate.
+    Qed.
+    
+    Lemma not_in_keys_find : forall e k,
+        ~ In k (keys e) -> find k e = None.
+    Proof.
+      intro e; induction e as [| [k v] e IHe];
+        intros ky Hky; unravel in *; auto.
+      destruct (find k e) as [vl |] eqn:Hfind;
+        destruct (HE ky k) as [Hkyk | Hkyk]; unravel in *; auto.
+      - apply IHe in Hky.
+        apply find_equiv_rel with (e := e) in Hkyk.
+        rewrite Hkyk in Hky.
+        rewrite Hky in Hfind. discriminate.
+      - apply Decidable.not_or in Hky as [Hkky Hkye].
+        apply IHe in Hkye.
+    Abort.
+    
+    Global Instance sub_env_reflexive : Reflexive sub_env.
+    Proof. firstorder. Qed.
+
+    Global Instance sub_env_transitive : Transitive sub_env.
+    Proof. firstorder. Qed.
+
+    Global Instance eq_env_reflexive : Reflexive eq_env.
+    Proof. firstorder. Qed.
+
+    Global Instance eq_env_symmetric : Symmetric eq_env.
+    Proof. firstorder. Qed.
+
+    Global Instance eq_env_transitive : Transitive eq_env.
+    Proof. firstorder. Qed.
+
+    Global Instance eq_env_equivalence : Equivalence eq_env.
+    Proof. firstorder. Qed.
+    
+    Global Instance sub_env_antisymmetric
+      : @Antisymmetric _ _ eq_env_equivalence sub_env.
+    Proof. firstorder. Qed.
+
+    Lemma find_none_bind_sub_env : forall e k v,
+        find k e = None -> sub_env e (bind k v e).
+    Proof.
+      unfold sub_env, bind;
+        intros e k v H k' v' Hkv'; simpl.
+      destruct_if; auto.
+      assert (Hfind: find k' e = find k e)
+        by auto using find_equiv_rel.
+      rewrite Hfind, H in Hkv'; discriminate.
+    Qed.
+
+    Lemma bind_sub_env_find_none : forall e k v,
+        sub_env e (bind k v e) -> find k e = None.
+    Proof.
+      unfold sub_env, bind;
+        intro e; induction e as [| [d t] e IHe]; simpl in *;
+          intros ky vl H; auto.
+    Abort.
+               
+    Lemma scope_shadow_sub_env :
+      forall e1 e2, sub_env e1 (scope_shadow e1 e2).
+    Proof.
+      unfold sub_env, scope_shadow;
+        intros e1 e2 k v Hkv.
+      induction e1 as [| [k1 v1] e1 IHe1];
+        simpl in *; auto; try discriminate.
     Qed.
   End Lemmas.
 End EnvDefs.
@@ -147,6 +264,12 @@ Section MapVals.
 End MapVals.
 
 Module EnvNotations.
+  Notation "e1 '⊆' e2"
+    := (sub_env e1 e2)
+         (at level 80, no associativity) : type_scope.
+  Notation "e1 '≝' e2"
+    := (eq_env e1 e2)
+         (at level 80, no associativity) : type_scope.
   Notation "'!{' env '}!'" := env (env custom p4env at level 99).
   Notation "x" := x (in custom p4env at level 0, x constr at level 0).
   Notation "'∅'" := (empty _ _) (in custom p4env at level 0, no associativity).
