deps/poulet4/lib/P4cub/BigStep/Properties.v
@@ -1,0 +1,33 @@
+Set Warnings "-custom-entry-overridden".
+Require Import Poulet4.P4cub.Syntax.Syntax Poulet4.P4cub.Envn
+        Poulet4.P4cub.BigStep.Value.Syntax
+        Poulet4.P4cub.BigStep.Semantics
+        Poulet4.P4cub.BigStep.IndPrincip.
+Import AllCubNotations Val.ValueNotations
+       Val.LValueNotations F.FieldTactics Step.
+
+Section Properties.
+  Lemma lv_update_sub_env : forall lv v ϵ,
+    ϵ ⊆ lv_update lv v ϵ.
+  Proof.
+    intro lv;
+      induction lv; intros v eps; simpl.
+    - (* not generally true. *) admit.
+  Abort.
+  
+  Context {tags_t : Type}.
+  Local Hint Resolve Env.scope_shadow_sub_env : core.
+  
+  Lemma stmt_big_step_sub_env :
+    forall ϵ ϵ' (s : Stmt.s tags_t) pkt pkt' fs cx sig,
+      ⟪ pkt , fs , ϵ , cx , s ⟫ ⤋ ⟪ ϵ' , sig , pkt' ⟫ -> ϵ ⊆ ϵ'.
+  Proof.
+    intros ? ? ? ? ? ? ? ? Hevals; induction Hevals;
+      try reflexivity;
+      try match goal with
+          | H12: ?e1 ⊆ ?e2, H23: ?e2 ⊆ ?e3
+            |- ?e1 ⊆ ?e3 => transitivity e2; assumption
+          end; auto.
+    - (* not generally true. *)
+  Abort.
+End Properties.
